commit

AP/AP/Defense/Defs.lean
@@ -11,11 +11,14 @@ structure Defense : Type where
 namespace Defense
 
 def st (dse : Defense) (d : DStrat) : DStrat :=
-  .mk # λ s => dse.f s |>.getD (d.f s)
+  .mk' # λ s => dse.f s |>.getD (d.f s)
 
-class WF (dse : Defense) : Prop where
-  h : ∀ s [sys.WF s], dse.cnd s → ∀ (a : AStrat) [a.WF], ∀ (d : DStrat) [d.WF] n,
-    (sys.simulate (Strat.f ⟨a, dse.st d⟩) s n).1.aPos ∉ dse.ps
+class ValidTr (dse : Defense) : Prop where
+  valid_tr : ∀ {s} [sys.WF s] {p}, dse.f s = some p → sys.validTr s p
+
+class WF (dse : Defense) extends dse.ValidTr where
+  not_mem_ps : ∀ {s} [sys.WF s], dse.cnd s → ∀ (a : AStrat) [a.WF],
+    ∀ (d : DStrat) [d.WF] n, (sys.simulate (Strat.f ⟨a, dse.st d⟩) s n).1.aPos ∉ dse.ps
 
 def sym (dse : Defense) (sym : sys.Symmetry) : Defense where
   cnd := λ s => dse.cnd # sym.fs s
