AP/AP/Defense/Basic.lean
@@ -2,13 +2,7 @@ import AP.AP.Defense.Defs
 
 namespace AP.Defense
 
-variable {dse : Defense}
-variable [wf : dse.WF]
-omit wf
-
-theorem wf_def : dse.WF ↔
-∀ s [sys.WF s], dse.cnd s → ∀ (a : AStrat) [a.WF], ∀ (d : DStrat) [d.WF] n,
-(sys.simulate (Strat.f ⟨a, dse.st d⟩) s n).1.aPos ∉ dse.ps := ⟨(·.1), (⟨·⟩)⟩
+variable {dse dse₁ dse₂ : Defense}
 
 instance : Inhabited Defense :=
   ⟨{cnd := λ _ => True, ps := ∅, f := λ _ => none}⟩
@@ -17,5 +11,20 @@ instance : Inhabited Defense :=
 theorem default_def : (default : Defense) =
 {cnd := λ _ => True, ps := ∅, f := λ _ => none} := rfl
 
-@[simp] instance : WF default := ⟨by simp⟩
-@[simp] instance {d} : (dse.st d).WF := by unfold st; infer_instance
+@[simp] instance : WF default where
+  valid_tr := by simp
+  not_mem_ps := by simp
+
+theorem valid_tr [H : dse.ValidTr] {s} [sys.WF s] {p} :
+dse.f s = some p → sys.validTr s p := H.1
+
+@[simp]
+instance [H : dse.ValidTr] {d : DStrat} [Hd : d.WF] : (dse.st d).WF := by
+  unfold st; rw [DStrat.wf_iff]; intro s hs
+  dsimp; cases h : dse.f s <;> simp; exact dse.valid_tr h
+
+theorem st_comm_of {d}
+(h : ∀ {s p₁ p₂}, dse₁.f s = some p₁ → dse₂.f s = some p₂ → p₁ = p₂) :
+dse₁.st (dse₂.st d) = dse₂.st (dse₁.st d) := by
+  ext s :2; simp [st]; cases h₁ : dse₁.f s <;> cases h₂ : dse₂.f s <;> simp
+  nm s₁ s₂; exact h h₁ h₂
